% -*- TeX-master: "master.tex" -*-
\section{Quantum Electrodynamics}
In deriving the Dirac equation, we formed Lorentz invariants out of Dirac spinors such as $\bar{\psi}\psi$.

Under the Lorentz group, $\bar{\psi}\psi$ is a scalar, $\bar{\psi}\gamma^\mu\psi$ is a 4-vector, so $\bar{\psi}\sla{\D}\psi$ is also a scalar.

We want a Lagrangian $\L$ invariant under the Lorentz group:
\begin{align*}
  \L=i\bar{\psi}\sla{\D}\psi-m\bar{\psi}\psi
\end{align*}
Equation of motion comes from the Principle of Least Action:
\begin{align*}
  \fdv{\L}{\bar{\psi}}=0\implies i\sla{D}\psi-m\psi=0
\end{align*}
Recall that the other term from the Euler-Lagrange is just $0$ since theres no derivatives of $\bar{\psi}$.

In addition to the Lorentz group, $\L$ is also invariant under the following symmetry:
\begin{align*}
  \psi&\to e^{iQ\theta}\psi\\
  \bar{\psi}&\to \bar{\psi}e^{-iQ\theta}
\end{align*}
Where $Q\in\mathbb{R}$, a $U(1)$ symmetry.

This is a \underline{global} symmetry, $\theta$ is the same over all spacetime. The symmetry group is $U(1)$. QED is introduced by demanding the $U(1)$ symmetry be \underline{local}, where $\theta=\theta(x)$ can change smoothly.

Clearly $m\bar{\psi}\psi$ is invariant:
\begin{align*}
  m\bar{\psi}\psi\to m\bar{\psi}e^{-iQ\theta(x)}e^{iQ\theta(x)}\psi
  =m\bar{\psi}\psi
\end{align*}
The other term:
\begin{align*}
  i\bar{\psi}\sla{\D}\psi\to
  \bar{\psi}e^{-iQ\theta(x)}\sla{\D}(e^{iQ\theta(x)}\psi)
  &=\bar{\psi}e^{-iQ\theta(x)}e^{iQ\theta(x)}\sla{\D}\psi
  +iQ\bar{\psi}\gamma^\mu\psi(\D_\mu\theta)\\
  &=i\bar{\psi}\sla{\D}\psi+i\bar{\psi}(iQ\sla{\D}\theta)\psi
\end{align*}
Is not invariant.

This is remedied by introducing a new field $A^\mu$, into the Lagrangian, and demanding $A^\mu$ transform in just the right way to cancel the offending term. Try the following:
\begin{align*}
  \L=i\bar{\psi}(+ieQ\sla{A})\psi
\end{align*}
Where $\sla{A}=A_\mu\gamma^\mu$, the photon field

The second term in the transformation of $i\bar{\psi}\sla{\D}\psi$ is cancelled if:
\begin{align*}
  A^\mu\to A^\mu-\frac1e\D^\mu\theta(x)
\end{align*}
This local transformation is called a \underline{gauge} transformation, and we say $\L$ is gauge invariant.

The field $A^\mu$ corresponds to the vector potential of the electromagnetic field, and $eQ$ is the electric charge of the fermion.
\begin{itemize}
\item $e$ is called the coupling constant $\alpha=e^2/4\pi\approx 1/137$ is the fine structure constant
\item $Q$ is the charge of particle in units of $e$, $Q=-1$ for electrons, and $Q=+\frac23$ for up quark, etc.
\end{itemize}
The quantum of the EM field is the photon. A mass term in $\L$ would be:
\begin{align*}
  -\frac12M^2A^\mu A_\mu
\end{align*}
But this is \underline{not} gauge invariant. We regard the masslessness of the photon as being a consequence of gauge invariance (although the inverse transformation is also reasonable).

The photon is a massless spin-1 particle and transforms as the $(1,0)\oplus(0,1)$ representation of the Lorentz group. It therefore as helicity $h=\pm1$.

Due to gauge invariance, $A_\mu\to A_\mu-\frac1e\D_\mu\theta$, we can always find a gauge (some $\theta(x)$) where:
\begin{align*}
  \D_\mu A^\mu=0
\end{align*}
This is called the Lorentz gauge, so called because of its manifest Lorentz invariance.

The photon field is:
\begin{align*}
  A^\mu(x)=\int\frac{\dd[3]{p}}{2E}\qty[
  e^{-ip\vdot x}a_\lambda\veps^\mu_\lambda(p)+
  e^{+ip\vdot x}a^\dag_\lambda\veps^{\mu*}_\lambda(p)
  ]
\end{align*}
Where $a,a^\dag$ are the destruction and creation operators for the photon, and $\veps^\mu_\lambda(p)$ is a four-vector which transforms as either the $(1,0)$ rep ($\lambda=+1$), or the $(0,1)$ rep ($\lambda=-1$) of the Lorentz group.

Recall $\psi(x)$:
\begin{align*}
  \psi(x)=\int\frac{\dd[3]{p}}{2E}\qty[
  e^{-ip\vdot x}a_\lambda u_\lambda(p)+
  e^{+ip\vdot x}b^\dag_\lambda v_\lambda(p)
  ]
\end{align*}
The Lorentz gauge condition implies:
\begin{align*}
  p_\mu\veps^\mu_\lambda(p)=0
\end{align*}
This means $\veps^\mu_\lambda$ is the Fourier transform of the photon field, and implies the photon is its own antiparticle.

The ``polarization vectors'' $\veps^\mu_\lambda$ for a photon with momentum $p^\mu=(E,0,0,E)$ are:
\begin{align*}
  \veps^\mu_+&=\frac1{\sqrt{2}}(0,1,i,0)\\
  \veps^\mu_-&=\frac1{\sqrt{2}}(0,1,-i,0)
\end{align*}

\begin{aside}
  Lorentz group (photon not massless) $\lambda=0,\pm1$, for a real photon we would have to remove $\lambda=0$. The radiation gauge, $A^0=0, \grad_i\vdot A^i$, $\lambda=\pm1$ manifestly.
\end{aside}

\subsection{Perturbation Theory}
QED is a weakly-coupled theory -- photons and electrons (or quarks) do not interact very strongly. To zeroth order they do not interact at all. Hence, one can regard interactions as perturbations of this simple picture. The outcome of treating QED perturbatively can be represented pictorially via Feynman diagrams. These ``Feynman rules'' are derived from quantum field theory. In practice, all one needs for simple calculations are the Feynman rules.

Lets draw the Feynman diagram for $e^+e^-\to\mu^+\mu^-$ then work out the details:
\begin{figure}[H]
  \centering
  \begin{tikzpicture}
    \begin{feynhand}
      \vertex (a) at (0,0);
      \vertex (e1) at (-1, 1) {$e^-$};
      \vertex (e2) at (-1,-1) {$e^+$};
      \vertex (m1) at (2.5, 1) {$\mu^-$};
      \vertex (m2) at (2.5,-1) {$\mu^+$};
      \vertex (b) at (1.5,0);
      \propag[mom=\(p_1\)] (e1) to (a);
      \propag[mom'=\(p_2\)] (e2) to (a);
      \propag[mom=\(p_3\)] (b) to (m1);
      \propag[mom'=\(p_4\)] (b) to (m2);
      \propag[bos, mom=\(q\)] (a) to (b);
    \end{feynhand}
    \draw[->] (3.0, 0.0) -- (4.0, 0.0);
    \node at (3.45, 0.2) {Time};
  \end{tikzpicture}
  \caption{Feynman Diagram for $e^+e^-\to\mu^+\mu^-$}
\end{figure}

\begin{aside}
  Many older books draw time going up. More modern notation has time flowing to the right. 
\end{aside}

The interaction ``vertex'' (seen below) comes from the Lagrangian:
\begin{align*}
  \L=i\bar{\psi}(\sla{\D}+ieQ\sla{A})\psi-m\bar{\psi}\psi
\end{align*}
\begin{figure}[H]
  \centering
  \begin{tikzpicture}
    \begin{feynhand}
      \vertex (a) at (0,0);
      \vertex (e1) at (-1, 1) {$e^-$};
      \vertex (e2) at (-1,-1) {$e^+$};
      \vertex (b) at (1.5,0) {$\gamma$}; 
      \propag (e1) to (a);
      \propag (e2) to (a);
      \propag[bos] (a) to (b);
    \end{feynhand}
  \end{tikzpicture}
  \caption{The interaction vertex}
\end{figure}
What does this mean?
\begin{itemize}
\item $\psi$ Destorys an $e^-$
\item $\bar{\psi}$ Destorys an $e^+$
\item $A^\mu$ creates a photon ($\gamma$)
\end{itemize}

We can ``read-off'' the Feynman rule for the interaction vertex: (Note that overall sign is convention, not all vertices are simple):
\begin{align*}
  \begin{tikzpicture}[baseline=-0.15cm]
    \begin{feynhand}
      \vertex (a) at (0,0);
      \vertex (e1) at (-1, 1) {$e^-$};
      \vertex (e2) at (-1,-1) {$e^+$};
      \vertex (b) at (1.5,0) {$\gamma$}; 
      \propag[fer] (e1) to (a);
      \propag[antfer] (e2) to (a);
      \propag[bos] (a) to (b);
    \end{feynhand}
  \end{tikzpicture}
  =-ieQ\gamma^\mu
\end{align*}
Where $Q=$ particle charge ($-1$ for $e^-$ and $e^+$).

The second ingredient we need is the ``propagator'' of the photon which mediates the interaction. This is not a real photon. A real photon is not kinematically allowed.
\begin{proof}
  Let the electron and positron 4-momenta respectively be:
  \begin{align*}
    p_1=(E,0,0,p)\qquad p_2=(E,0,0,-p)
  \end{align*}
  And that they are colliding head-on (in c.o.m.\ frame) in an experiment (BEPC, Tristan, CESR, SLAC, LEP, etc.)
  The photon momentum is the sum of these two:
  \begin{align*}
    q_{\gamma}&=p_1+p_2=(2E,0,0,0)\\
    \implies q_{\gamma}^2=4E^2\neq 0
  \end{align*}
  A real photon would have $q^2=0$ always. 
\end{proof}

The interaction is mediated by a ``virtual'' photon (a particle \underline{not} ``on the mass shell'', i.e.\ $q^2\neq m^2$). These ``particles'' do not actually exist in the same sense that real photons (w/ $q^2=0$) do. Also $q^2$ is \underline{not} constrained to be greater than $0$ in general (though it is here).

What is the time scale of this interaction? Dimensional analysis says:
\begin{align*}
  t\sim\frac1{\sqrt{q^2}}\sim\frac1{2E}
\end{align*}
The minimum (threshold) energy for this interaction is that $2E\sim\SI{200}{\MeV}$ Hence $t$ is about:
\begin{align*}
  t\sim\frac{\hbar c}{2Ec}\sim 10^{-23}\text{s}
\end{align*}

When a virtual particle appears in a Feynman diagram, this corresponds to a propagator:
\begin{align*}
  \text{spin 0}\quad
  \begin{tikzpicture}[baseline=-0.10cm]
    \begin{feynhand}
      \vertex (a) at (0,0);
      \vertex (b) at (1.5,0); 
      \propag[sca, mom=\(p\)] (a) to (b);
    \end{feynhand}
  \end{tikzpicture}
  &=\frac{i}{p^2-m^2}\\
  \text{spin }\frac12\quad
  \begin{tikzpicture}[baseline=-0.10cm]
    \begin{feynhand}
      \vertex (a) at (0,0);
      \vertex (b) at (1.5,0); 
      \propag[fer, mom=\(p\)] (a) to (b);
    \end{feynhand}
  \end{tikzpicture}
  &=\frac{i}{\sla{p}-m}=\frac{i(\sla{p}+m)}{p^2-m^2}\\
  \text{(massless) spin 1}\quad
  \begin{tikzpicture}[baseline=-0.10cm]
    \begin{feynhand}
      \vertex (a) at (0,0);
      \vertex (b) at (1.5,0); 
      \propag[bos, mom=\(p\)] (a) to (b);
    \end{feynhand}
  \end{tikzpicture}
  &=\frac{i(-g^{\mu\nu}+p^\mu p^\nu/p^2)}{p^2}
\end{align*}
\begin{remark}
  The charge arrow on the fermion above is defined such that the direction of motion of the \emph{particle} is the direction of the charge arrow. \emph{Antiparticles} go backward in time.
\end{remark}

The numerators of the propagators come from summing over helicities:
\begin{align*}
  \sum_{\lambda=\pm}u_\lambda\bar{u}_\lambda&=\sla{p}+m\\
  \sum_{\lambda=\pm,0}\veps^\mu_\lambda\bar{\veps}^\nu_\lambda&=
  -g^{\mu\nu}+\frac{p^\mu p^\nu}{p^2}
\end{align*}

The photon propagator looks complicated, but we will see that the second term will not contribute in practice in either of QED or QCD.

Lets now turn the pictogram into an actual calculation of the scattering amplitude:
\begin{figure}[H]
  \centering
  \begin{tikzpicture}[scale=2.0]
    \begin{feynhand}
      % vertices
    \vertex (p11) at (-1,1) {$e^-$};
    \vertex (p12) at (-1,-1) {$e^+$};
    \vertex (p21) at (3,1) {$\mu^-$};
    \vertex (p22) at (3,-1) {$\mu^+$};
    \vertex (a) at (0,0);
    \vertex (b) at (2,0);
    % particles
    \propag [fer, mom=\(p_1\)] (p11) to (a);
    \propag [antfer, mom'=\(p_2\)] (p12) to (a);
    \propag [fer, mom=\(p_3\)] (b) to (p21);
    \propag [antfer, mom'=\(p_4\)] (b) to (p22);
    % propagator
    \propag [bos, mom=\(q\)] (a) to [edge label'=\(\gamma\)] (b);
    \end{feynhand}
  \end{tikzpicture}
  \caption{$e^+e^-\to\mu^+\mu^-$}
  \label{fig:feynman}
\end{figure}
The arrows on the actual edges indicate charge or ``fermion'' flow, read the spinor chain opposite in the direction of these arrows, for example, the left chain would be read as:
\begin{align*}
  \bar{v}(p_2)(-ieQ_e\gamma^\mu)u(p_1)
\end{align*}
And the right chain would read as:
\begin{align*}
  \bar{u}(p_3)(-ieQ_\mu\gamma^\nu)v(p_4)
\end{align*}
The last thing to get is the propagator, then we can write out $\M$, the matrix element:
\begin{align*}
  i\M=&(-ieQ_e)\bar{v}(p_2)\gamma^\mu u(p_1)\\
  \times&\frac{i}{q^2}\qty(-g_{\mu\nu}+\frac{q_\mu q_\nu}{q^2})\\
  \times&(-ieQ_\mu)\bar{u}(p_3)\gamma^\nu v(p_4)
\end{align*}
$\M$ is the amplitude, we will square $\M$ to get the probability that feeds into the cross section or particle decay width.

Lets first show that the second term in the photon propagator does not contribute:
\begin{proof}
  Consider what is actually being calculated:
  \begin{align*}
    \bar{v}(p_2)\gamma^\mu u(p_1)q_\mu=\bar{v}(p_2)\sla{q}u(p_1)
  \end{align*}
  By conservation of momentum, we know that $q=p_1+p_2$:
  \begin{align*}
    \bar{v}(p_2)\sla{q}u(p_1)=\bar{v}(p_2)(\sla{p}_1+\sla{p}_2)u(p_1)
  \end{align*}
  Note that on each side we can use the momentum-space Dirac equation, namely that:
  \begin{align*}
    \sla{p}_1u(p_1)&=m u(p_1)\\
    \bar{v}(p_2)\sla{p}_2&=-m\bar{v}(p_2)
  \end{align*}
  This gives a factor of $m$ and $-m$ in the parentheses:
  \begin{align*}
    \bar{v}(p_2)(\sla{p}_1+\sla{p}_2)u(p_1)
    =\bar{v}(p_2)(m-m)u(p_1)=0
  \end{align*}
  The factors $\bar{v}(p_2)\gamma^\mu u(p_1)$ and $\bar{u}(p_3)\gamma^\nu v(p_4)$ are called the fermion current, $j^\mu$, and the fact that $q_\mu j^\mu=0$ is called current conservation. This is directly from Maxwell's equations in covariant form.
\end{proof}
Thus our matrix element can be reduced drastically:
\begin{align*}
  i\M=&(-ieQ_e)\bar{v}(p_2)\gamma^\mu u(p_1)
  \times-\frac{i}{q^2}g_{\mu\nu}
  \times(-ieQ_\mu)\bar{u}(p_3)\gamma^\nu v(p_4)\\
  =&i\frac{e^2Q_e Q_\mu}{q^2}\bar{v}(p_2)\gamma^\mu u(p_1)
  g_{\mu\nu}\bar{u}(p_3)\gamma^\nu v(p_4)\\
  =&i\frac{e^2Q_e Q_\mu}{q^2}\bar{v}(p_2)\gamma^\mu u(p_1)
  \bar{u}(p_3)\gamma_\mu v(p_4)
\end{align*}
Now we can square the amplitude: $\abs{\M}^2=\M\M^*$:
\begin{align*}
  \abs{\M}^2=&e^4Q_e^2Q_\mu^2q^{-4}\bar{v}p_2\gamma^\mu u(p_1)
  {(\bar{v}(p_2)\gamma^\nu u(p_1))}^*\\
  \times&\bar{u}(p_3)\gamma_\mu v(p_4)
  {(\bar{u}(p_3)\gamma_\nu v(p_4))}^*
\end{align*}
Notice that the factor of $\M^*$ has a different index on it. We can also trivially turn the complex conjugate into a conjugate transpose as we are dealing with scalars in Dirac-space:
\begin{align*}
  {(\bar{v}(p_2)\gamma^\nu u(p_1))}^*&={(\bar{v}(p_2)\gamma^\nu u(p_1))}^\dag\\
  =u^\dag(p_1){(\gamma^\nu)}^\dag{(\gamma^0)}^\dag v(p_2)
  &=u^\dag(p_1)\gamma^0\gamma^\nu\gamma^0\gamma^0 v(p_2)\\
  &=\bar{u}(p_1)\gamma^\nu v(p_2)
\end{align*}

Often the colliding beams at these experiments are unpolarized, so it is useful to average over helicities:
\begin{align*}
  \frac12\frac12\sum_{\lambda=\pm}\sum_{\lambda'=\pm}
  \bar{v}_{\lambda'}(p_2)\gamma^\mu u_\lambda(p_1)
  \bar{u}_{\lambda}(p_1)\gamma^\nu v_{\lambda'}(p_2)
\end{align*}
We now need to make use of the matrix-nature of this expression. Since the expression is a complex number, we have:
\begin{align*}
  \sum_i M_{ii}=\Tr[M_{ij}]
\end{align*}
Because of this, we can move $\bar{v}_{\lambda'}$ to the end of the chain:
\begin{align*}
  \frac12\frac12\sum_{\lambda=\pm}\sum_{\lambda'=\pm}\Tr[
  \gamma^\mu u_\lambda(p_1)\bar{u}_{\lambda}(p_1)
  \gamma^\nu v_{\lambda'}(p_2)\bar{v}_{\lambda'}(p_2)]
\end{align*}
Now we can use:
\begin{align*}
  \sum_{\lambda=\pm}u_\lambda(p_1)\bar{u}_\lambda(p_1)&=\sla{p}_1+m\\
  \sum_{\lambda'=\pm}v_\lambda(p_2)\bar{v}_\lambda(p_2)&=\sla{p}_2-m
\end{align*}
This is called ``Casimir's Trick'', and we can now use the trace ``theorems'':
\begin{align*}
  \acomm{\gamma^\mu}{\gamma^\nu}&=2g^{\mu\nu}\\
  \Tr[\gamma^\mu]&=0\\
  \Tr[\gamma^\mu\gamma^\nu]&=4g^{\mu\nu}\\
  \Tr[\gamma^\mu\gamma^\nu\gamma^\sigma\gamma^\rho]&=
  4[g^{\mu\nu}g^{\sigma\rho}+g^{\nu\sigma}g^{\mu\rho}-g^{\nu\rho}g^{\mu\sigma}]\\
  \Tr[\text{odd \# of $\gamma$'s}]&=0
\end{align*}
So our trace is fairly easy:
\begin{align*}
  \frac14\Tr[\gamma^\mu(\sla{p}_1+m_e)\gamma^\nu(\sla{p}_2-m_e)]
  &=\frac14\qty{\Tr[\gamma^\mu\sla{p}_1\gamma^\nu\sla{p_2}]
    -m_e^2\Tr[\gamma^\mu\gamma^\nu]}\\
  &=\frac144\qty{p_{1\rho}p_{2\sigma}
    (g^{\mu\rho}g^{\nu\sigma}+g^{\nu\rho}g^{\mu\sigma}-g^{\mu\nu}g^{\rho\sigma})
    -m_e^2g^{\mu\nu}}\\
  &=p_1^\mu p_2^\nu+p_1^\nu p_2^\mu-p_1\vdot p_2g^{\mu\nu}-m_e^2g^{\mu\nu}
\end{align*}
Similarly, the helicities of the final-state fermions are often unobserved, so we can sum over all helicities. 