\documentclass[12pt]{article}

\title{\vspace{-3em}Fun With Integrals}
\author{Michael Cardiff}
\date{\today}

%% science symbols 
\usepackage{amsmath}
\usepackage{amssymb}
\usepackage{physics}

%% general pretty stuff
\usepackage{bm}
\usepackage{enumitem}
\usepackage{float}
\usepackage{graphicx}
\usepackage[margin=1in]{geometry}

% figures
\graphicspath{ {./figs/} }

\newcommand{\fig}[3]
{
  \begin{figure}[H]
    \centering
    \includegraphics[width=#1cm]{#2}
    \caption{#3}
  \end{figure}
}

\newcommand{\figref}[4]
{
  \begin{figure}[H]
    \centering
    \includegraphics[width=#1cm]{#2}
    \caption{#3}
    \label{#4}
  \end{figure}
}

\renewcommand{\L}{\mathcal{L}}

\begin{document}
\maketitle
In class we wanted to compute the integral:
\begin{align*}
  \int_0^\infty\dd{x}\frac{x^3}{e^x-1}
\end{align*}
Recall the $3$ comes from the fact that we are computing the heat capacity for a 3-D solid, if we were to compute this for an $n$-D solid, we would have the following integral:
\begin{align*}
  \int_0^\infty\dd{x}\frac{x^n}{e^x-1}
\end{align*}
We can use the geometric series of the following term to make this integral simpler:
\begin{align*}
  \sum_{s=0}^{\infty}e^{-sx}=\frac{e^x}{e^x-1}
\end{align*}
We can use this to substitute in our integral:
\begin{align*}
  \int_0^\infty\dd{x}\frac{x^n}{e^x-1}=
  \int_0^\infty\dd{x}x^ne^{-x}\sum_{s=0}^\infty e^{-sx}
\end{align*}
By the magic of Fubini's theorem (supposedly) we can interchange the integral and the sum:
\begin{equation}
  \sum_{s=0}^\infty\int_0^\infty\dd{x}x^ne^{-(s+1)x}\label{bruh}
\end{equation}
Recall the definitions of the following special functions in math:
\begin{align*}
  \zeta(s)&=\sum_{n=1}^\infty\frac{1}{n^s}\\
  \Gamma(n+1)&=\int_0^\infty\dd{x}x^ne^{-x}
\end{align*}
If we introduce a substitution into \eqref{bruh} we should find a gamma function:
\begin{gather*}
  \alpha = (s+1)x\\
  \dd{\alpha} = (s+1)\dd{x}\\
  I=\sum_{s=0}^\infty\int_0^\infty\frac{\dd{\alpha}}{s+1}\qty(\frac{\alpha}{s+1})^n
  e^{-\alpha}
\end{gather*}
We can then turn our end result into:
\begin{align*}
  I=\sum_{s=0}^\infty\frac{1}{(s+1)^{n+1}}
  \int_0^\infty\dd{\alpha}\alpha^ne^{-\alpha}
\end{align*}
The integral is not dependent on $s$ at all, so it and the sum are independent, clearly the integral is the gamma function:
\begin{align*}
  I=\sum_{s=0}^\infty\frac{1}{(s+1)^{n+1}}\Gamma(n+1)
\end{align*}
Readjusting the sum index allows it to match the definition of $\zeta$:
\begin{align*}
  I=\sum_{t=1}^\infty\frac{1}{t^{n+1}}\Gamma(n+1)=\zeta(n+1)\Gamma(n+1)
\end{align*}
\end{document}